Lazy rand impl

theories/coneris/examples/lazy_rand/lazy_rand_impl.v
@@ -3,6 +3,7 @@ From clutch.coneris Require Import coneris abstract_tape hocap_rand_alt lock laz
 
 Set Default Proof Using "Type*".
 
+
 (* Section lemmas. *)
 (*   Context `{!inG Σ (excl_authR (optionO (prodO natO natO)))}. *)
 
@@ -54,8 +55,8 @@ Section impl.
                                                 | SOME "x'" =>
                                                     "x'"
                                                 | NONE =>
-                                                    let: "x'" := SOME (rand_tape "α", "tid") in 
-                                                    "x" <- "x'";;
+                                                    let: "x'" := (rand_tape "α", "tid") in 
+                                                    "x" <- SOME "x'";;
                                                     "x'"
                                                 end) in
                                  release "l" ;;
@@ -94,12 +95,20 @@ Section impl.
     match n with
     | Some (n1, n2) => SOMEV (#n1, #n2)%V
     | None => NONEV end.     
+
+  Definition rand_frag (res tid:nat) (γ:gname):=(() ↪[γ]□ Some (res, tid))%I.
+  
+  Definition option_duplicate (n:option (nat* nat)) γ:=
+    match n with
+    | Some (n1, n2) => rand_frag n1 n2 γ
+    | None => (⌜True⌝)%I
+    end.
   
   Definition rand_auth (n:option (nat*nat)) γ :=
     (ghost_map_auth γ 1 (option_to_gmap n) ∗
+     option_duplicate n γ ∗
      ⌜option_valid n⌝)%I.
 
-  Definition rand_frag (res tid:nat) (γ:gname):=(() ↪[γ]□ Some (res, tid))%I.
   
   Definition lazy_rand_inv N c P{HP: ∀ n, Timeless (P n)}  γ_tape γ_view γ_lock :=
     (∃ lk (l:loc),
@@ -117,7 +126,17 @@ Section impl.
           ↯ (ε2 n) ∗
           rand_tape_auth (<[α:=Some (fin_to_nat n)]>m) γ ∗
           rand_tape_frag α (Some (fin_to_nat n)) γ).
-  Admitted.
+    iIntros (???) "(%&%&->&#[? Hinv]&#?) [Htokens Htauth] [Htape Hfrag] Herr".
+    iDestruct (abstract_tapes_agree with "[$][$]") as "%H'".
+    rewrite lookup_fmap in H'. apply fmap_Some_1 in H'.
+    destruct H' as (?&Hsome&?). simplify_eq.
+    iMod (rand_tapes_presample with "[$][$][$]") as "(%&Htape&?)"; try done.
+    iMod (abstract_tapes_presample with "[$][$]") as "[? H]".
+    iFrame. iModIntro.
+    iSplitL "Htokens".
+    - by rewrite dom_insert_lookup_L.
+    - by rewrite fmap_insert.
+  Qed.
 
   Lemma lazy_rand_presample_impl N c P {HP: ∀ n, Timeless (P n)} γ γ_view γ_lock Q
     E  :
@@ -130,7 +149,12 @@ Section impl.
     state_update E E (
         ∃ m m', Q m m'
       ).
-  Admitted.
+    iIntros (?) "(%&%&->&#[Hinv ?]&#?) Hvs".
+    iInv "Hinv" as ">(%&?)" "Hclose".
+    iMod ("Hvs" with "[$]") as "(%&?&?)".
+    iMod ("Hclose" with "[$]") as "_".
+    by iFrame.
+  Qed.
 
   Lemma lazy_rand_init_impl N P {HP: ∀ n, Timeless (P n)} :
     {{{ P None }}}
@@ -139,7 +163,27 @@ Section impl.
           ∃ γ γ_view γ_lock, 
             lazy_rand_inv N c P γ γ_view γ_lock }}}.
   Proof.
-  Admitted.
+    iIntros (Φ) "HP HΦ". iApply pgl_wp_fupd.
+    rewrite /init_lazy_rand_prog.
+    wp_pures.
+    wp_alloc x as "Hx".
+    wp_pures.
+    iMod (ghost_map_alloc (<[():=None]> ∅)) as "(%&Hm&_)".
+    wp_apply (newlock_spec (∃ res, P res ∗ rand_auth res _ ∗ _↦(option_to_val res))%I
+                           with "[$HP $Hx $Hm //]"
+             ).
+    iIntros (??) "#Hlock".
+    wp_pures.
+    iMod (rand_inv_create_spec) as "(%&#Hrand)"; last first.
+    - iMod (abstract_tapes_alloc ∅) as "(%&Hm&_)".
+      iMod (inv_alloc _ _ (∃ m, rand_tape_auth m (_,_)) with "[Hm]") as "#Hinv".
+      { iNext. iExists ∅. rewrite /rand_tape_auth. rewrite fmap_empty.
+        iFrame. by rewrite dom_empty_L. }
+      iApply "HΦ". iFrame "Hlock".
+      rewrite /abstract_lazy_rand_inv. iExists (_,_).
+      by iFrame "Hrand Hinv".
+    - done.
+  Qed.
 
   Lemma lazy_rand_alloc_tape_impl N c P {HP: ∀ n, Timeless (P n)} γ_tape γ_view γ_lock Q:
   {{{ lazy_rand_inv N c P γ_tape γ_view γ_lock ∗
@@ -148,26 +192,84 @@ Section impl.
       allocate_tape_prog #()
       {{{ (α: val), RET α; rand_tape_frag α None γ_tape ∗ Q α }}}.
   Proof.
-  Admitted.
+    iIntros (Φ) "[(%&%&->&#[Hinv ?]&_) Hvs] HΦ".
+    rewrite /allocate_tape_prog.
+    wp_pures.
+    iApply pgl_wp_fupd.
+    wp_apply (rand_allocate_tape_spec with "[//]") as (α) "[Htoken Hrand]"; first done.
+    iInv "Hinv" as ">(%m&Htokens&Hauth)" "Hclose".
+    iAssert (⌜α∉dom m⌝)%I as "%".
+    { iIntros "%H".
+      rewrite big_sepS_elem_of_acc; last done.
+      iDestruct "Htokens" as "[? ?]".
+      iApply (rand_token_exclusive with "[$][$]").
+    }
+    iMod ("Hvs" with "[//]") as "HQ".
+    iMod (abstract_tapes_new with "[$]") as "[Hauth Htape]"; last first.
+    - iMod ("Hclose" with "[Hauth Htoken Htokens]").
+      + iExists (<[_:=_]> _). rewrite /rand_tape_auth.  rewrite fmap_insert. iFrame.
+        rewrite dom_insert_L big_sepS_insert; last done.
+        iFrame.
+      + iApply "HΦ". by iFrame.
+    - rewrite lookup_fmap. apply not_elem_of_dom_1 in H. by rewrite H.
+  Qed.
 
   Lemma lazy_rand_spec_impl N c P {HP: ∀ n, Timeless (P n)} γ_tape γ_view γ_lock Q1 Q2 α (v:nat) (tid:nat):
   {{{ lazy_rand_inv N c P γ_tape γ_view γ_lock ∗
-      ( ∀ n m, P n -∗ rand_auth n γ_view -∗ rand_tape_auth m γ_tape -∗ state_update (⊤∖↑N.@"tape") (⊤∖↑N.@"rand")
+      ( ∀ n m, P n -∗ rand_auth n γ_view -∗ rand_tape_auth m γ_tape -∗ state_update (⊤∖↑N.@"tape") (⊤∖↑N.@"tape")
              match n with
              | Some (res, tid') => P n ∗ rand_auth n γ_view ∗ rand_tape_auth m γ_tape ∗ Q1 res tid'
              | None => ∃ n', rand_tape_frag α (Some n') γ_tape ∗ rand_tape_auth (<[α:=Some n']> m) γ_tape ∗
-                              (∀ (m':gmap val (option nat)), ⌜m'!!α=(Some (Some n'))⌝
+                              (rand_tape_frag α None γ_tape
                                       ={⊤∖↑N.@"tape"}=∗  P (Some (n', tid)) ∗ rand_auth (Some (n', tid)) γ_view ∗ Q2 n' tid)
              end                                        
       )
   }}}
-      c α #tid
+      lazy_read_rand_prog c α #tid
       {{{ (res' tid':nat), RET (#res', #tid')%V;  (Q1 res' tid' ∨
-                                  rand_tape_frag α None γ_tape ∗ Q2 res' tid'
+                                                   Q2 res' tid'
                                 )
       }}}.
   Proof.
-  Admitted.
+    iIntros (Φ) "[(%&%&->&#[Hinv ?]&#Hlock) Hvs] HΦ".
+    rewrite /lazy_read_rand_prog. wp_pures.
+    wp_apply (acquire_spec with "[$]") as "[Hl (%res&HP&(Hauth & Hfrag & %Hvalid)&Hloc)]".
+    wp_pures.
+    wp_load.
+    iApply state_update_pgl_wp.
+    iInv ("Hinv") as ">(%&Htokens&Htauth)" "Hclose".
+    iMod ("Hvs" with "[$][$Hauth $Hfrag//][$]") as "Hcont".
+    destruct res as [[]|].
+    - iDestruct "Hcont" as "(HP&Hauth &Htauth&HQ)".
+      iMod ("Hclose" with "[$Htauth]") as "_".
+      iModIntro. wp_pures.
+      wp_apply (release_spec with "[$Hlock $Hl $HP $Hloc $Hauth]").
+      iIntros. wp_pures.
+      iApply "HΦ". by iFrame.
+    - iDestruct "Hcont" as "(%&[Ht Htfrag] &[Htokens Htauth] & Hvs)".
+      iMod ("Hclose" with "[$Htauth $Htokens]") as "_".
+      iModIntro. wp_pures.
+      wp_apply (rand_tape_spec_some with "[$]") as "Htape"; first done.
+      iApply fupd_pgl_wp.
+      iInv ("Hinv") as ">(%&Htokens&Htauth)" "Hclose".
+      iDestruct (abstract_tapes_agree with "[$][$]") as "%Hsome".
+      apply lookup_fmap_Some in Hsome.
+      destruct Hsome as ([x|]&?&Hsome); simplify_eq.
+      iMod (abstract_tapes_pop with "[$][$]") as "[Hauth Htape']".
+      iMod ("Hvs" with "[$]") as "(HP&Hrand&HQ)".
+      iMod ("Hclose" with "[Hauth Htokens]") as "_".
+      { iExists (<[_:=None]>_).
+        rewrite /rand_tape_auth. rewrite fmap_insert.
+        rewrite dom_insert_lookup_L; last done. iFrame.
+      }
+      iModIntro.
+      wp_pures.
+      wp_store.
+      wp_pures.
+      wp_apply (release_spec with "[$Hlock $Hl $HP $Hloc $Hrand]").
+      iIntros. wp_pures. iModIntro. iApply "HΦ".
+      iFrame.
+  Qed.
   
   Program Definition lazy_rand_impl : lazy_rand val_size :=
     {| init_lazy_rand := init_lazy_rand_prog;
@@ -186,18 +288,49 @@ Section impl.
     |}
   .
   Next Obligation.
-  Admitted.
+    intros [[]|]?; rewrite /rand_auth/=; apply _.
+  Qed.
   Next Obligation.
-  Admitted.
+    rewrite /rand_tape_frag/=.
+    iIntros (???) "[??]".
+    iDestruct (rand_tapes_valid with "[$]") as "%H".
+    by rewrite Forall_singleton in H.
+  Qed.
   Next Obligation.
-  Admitted.
+    rewrite /rand_tape_frag.
+    iIntros (????) "[??][??]".
+    iApply (rand_tapes_exclusive with "[$][$]").
+  Qed.
   Next Obligation.
-  Admitted.
+    rewrite /rand_tape_auth/rand_tape_frag.
+    iIntros (?? x ?) "[??][??]".
+    iDestruct (abstract_tapes_agree with "[$][$]") as "%Hsome".
+    apply lookup_fmap_Some in Hsome.
+    by destruct Hsome as ([[]|]&?&Hsome); destruct x; simplify_eq.
+  Qed.
   Next Obligation.
-  Admitted.
+    rewrite /rand_auth.
+    iIntros (???) "[??][??]".
+    iDestruct (ghost_map_auth_valid_2 with "[$][$]") as "[%?]".
+    done.
+  Qed.
   Next Obligation.
-  Admitted.
+    rewrite /rand_auth/rand_frag.
+    iIntros (????)"[H ?]H'".
+    iCombine "H H'" gives "%H".
+    destruct n; simpl in H; simplify_eq.
+    rewrite /option_to_gmap in H. rewrite lookup_insert in H.
+    by simplify_eq.
+  Qed.
   Next Obligation.
-  Admitted.
+    iIntros ([]?) "(?&#?&?)".
+    iFrame. by iSplit.
+  Qed.
+  Next Obligation.
+    rewrite /rand_frag.
+    iIntros (?????) "H H'".
+    iCombine "H H'" gives "%".
+    iPureIntro. naive_solver.
+  Qed.
   
 End impl.
